theories/LogicalRelation/Definition/W.v
@@ -1,7 +1,7 @@
 (** * LogRel.LogicalRelation.Definition.Sig : Definition of the logical relation for dependent sums *)
 From Coq Require Import CRelationClasses.
 From LogRel Require Import Utils Syntax.All GenericTyping.
-From LogRel.LogicalRelation.Definition Require Import Prelude Poly.
+From LogRel.LogicalRelation.Definition Require Import Prelude Poly Ne.
 
 Set Primitive Projections.
 Set Universe Polymorphism.
@@ -11,83 +11,106 @@ Set Polymorphic Inductive Cumulativity.
 (** ** Reducibility of dependent sum types *)
 
 Definition WRedTyPack `{ta : tag} `{WfContext ta} `{WfType ta} `{ConvType ta} `{RedType ta} :=
-  ParamRedTyPack (T:=tSig).
+  ParamRedTyPack (T:=tW).
 
-Definition SigRedTyAdequate@{i j} `{ta : tag} `{WfContext ta} `{WfType ta} `{ConvType ta} `{RedType ta}
-    {Γ : context} {A B : term} (R : RedRel@{i j}) (ΣA : SigRedTyPack@{i} Γ A B)
-  : Type@{j} := PolyRedPackAdequate R ΣA.
+Definition WRedTyAdequate@{i j} `{ta : tag} `{WfContext ta} `{WfType ta} `{ConvType ta} `{RedType ta}
+    {Γ : context} {A B : term} (R : RedRel@{i j}) (WA : WRedTyPack@{i} Γ A B)
+  : Type@{j} := PolyRedPackAdequate R WA.
 
-Module SigRedTyPack := ParamRedTyPack.
+Module WRedTyPack := ParamRedTyPack.
 
-Inductive isLRPair `{ta : tag} `{WfContext ta}
-  `{WfType ta} `{ConvType ta} `{RedType ta} `{Typing ta} `{ConvTerm ta} `{ConvNeuConv ta}
-  {Γ : context} {A B : term} (ΣA : SigRedTyPack Γ A B) : term -> Type :=
-| PairLRPair : forall (A' B' a b : term)
-      (wtydom : [Γ |- A'])
-      (convtydom : [Γ |- SigRedTyPack.domL ΣA ≅ A'])
-      (wtycod : [Γ |- B'[a..]])
-      (convtycod : [Γ |- (SigRedTyPack.codL ΣA)[a..] ≅ B'[a..]])
-  (rfst : forall {Δ} (ρ : Δ ≤ Γ) (h : [ |- Δ ]),
-      [ΣA.(PolyRedPack.shpRed) ρ h | Δ ||- a⟨ρ⟩ ≅ a⟨ρ⟩ : (SigRedTyPack.domL ΣA)⟨ρ⟩])
-  (rsnd : forall {Δ} (ρ : Δ ≤ Γ) (h : [ |- Δ ]),
-      [ΣA.(PolyRedPack.posRed) ρ h (rfst ρ h) | Δ ||- b⟨ρ⟩ ≅ b⟨ρ⟩ : (SigRedTyPack.codL ΣA)[a⟨ρ⟩ .: (ρ >> tRel)] ]),
 
-  isLRPair ΣA (tPair A' B' a b)
-
-| NeLRPair : forall p : term, [Γ |- p ~ p : SigRedTyPack.outTy ΣA] -> isLRPair ΣA p.
-
-Module SigRedTmEq.
-
-  Record SigRedTm `{ta : tag} `{WfContext ta}
+Module WRedTmEq.
+Section WRedTmEq.
+  Context `{ta : tag} `{WfContext ta}
     `{WfType ta} `{ConvType ta} `{RedType ta}
     `{Typing ta} `{ConvTerm ta} `{ConvNeuConv ta} `{RedTerm ta}
-    {Γ : context} {A B : term} {ΣA : SigRedTyPack Γ A B} {t : term}
-  : Type := {
-    nf : term;
-    red : [ Γ |- t :⤳*: nf : SigRedTyPack.outTy ΣA ];
-    ispair : isLRPair ΣA nf;
-  }.
+    {Γ : context} {A B : term} {WA : WRedTyPack Γ A B}.
 
-  Arguments SigRedTm {_ _ _ _ _ _ _ _ _ _ _ _}.
+  Inductive WRedTmEq {Δ} {ρ : Δ ≤ Γ} : term -> term -> Type :=
+  | Build_WRedTmEq {t u}
+      (nfL : term)
+      (nfR : term)
+      (redL : [ Δ |- t :⤳*: nfL : (WRedTyPack.outTy WA)⟨ρ⟩ ])
+      (redR : [ Δ |- u :⤳*: nfR : (WRedTyPack.outTy WA)⟨ρ⟩ ])
+      (* really useful ? *)
+      (eq : [ Γ |- nfL ≅ nfR : (WRedTyPack.outTy WA)⟨ρ⟩ ])
+      (prop : @WPropEq Δ ρ nfL nfR) : WRedTmEq t u
 
-  Lemma whnf `{GenericTypingProperties} {Γ A B} {ΣA : SigRedTyPack Γ A B} {t} :
-    forall (red : SigRedTm ΣA t), whnf (nf red).
+  with WPropEq {Δ} {ρ : Δ ≤ Γ} : term -> term -> Type :=
+  | supReq {A A' B B' a a' k k'}
+    (* (wtA : [Γ |- A])
+    (wtA' : [Γ |- A']) *)
+    (convtyA : [Γ |- WRedTyPack.domL WA ≅ A])
+    (convtyA' : [Γ |- WRedTyPack.domL WA ≅ A'])
+    (convtyB : [Γ ,, WRedTyPack.domL WA |- WRedTyPack.codL WA ≅ B])
+    (convtyB' : [Γ ,, WRedTyPack.domL WA |- WRedTyPack.codL WA ≅ B'])
+    (Ra : forall {Ξ} (ρ' : Ξ ≤ Δ) (wfΞ : [ |- Ξ ]),
+      [WA.(PolyRedPack.shpRed) (ρ' ∘w ρ) wfΞ | _ ||- a⟨ρ'⟩ ≅ a'⟨ρ'⟩ : _ ≅ _])
+    (Rk : forall {Ξ b b'} (ρ' : Ξ ≤ Δ) (wfΞ : [ |- Ξ ]),
+      [WA.(PolyRedPack.posRed) (ρ' ∘w ρ) wfΞ (Ra ρ' wfΞ) | _ ||- b ≅ b' : _ ≅ _] ->
+      @WRedTmEq Ξ (ρ' ∘w ρ) (tApp k⟨ρ'⟩ b) (tApp k'⟨ρ'⟩ b')) :
+    WPropEq (tSup A B a k) (tSup A' B' a' k')
+  | neReq {ne ne'} :
+    [Γ ||-NeNf ne ≅ ne' : (WRedTyPack.outTy WA)⟨ρ⟩] -> WPropEq ne ne'.
+
+Scheme WRedTmEq_mut_rect := Induction for WRedTmEq Sort Type with
+    WPropEq_mut_rect := Induction for WPropEq Sort Type.
+
+Combined Scheme _WRedInduction from
+  WRedTmEq_mut_rect,
+  WPropEq_mut_rect.
+
+Combined Scheme _WRedEqInduction from
+  WRedTmEq_mut_rect,
+  WPropEq_mut_rect.
+
+Let _WRedEqInductionType :=
+  ltac:(let ind := fresh "ind" in
+      pose (ind := _WRedEqInduction);
+      let ind_ty := type of ind in
+      exact ind_ty).
+
+Let WRedEqInductionType :=
+  ltac: (let ind := eval cbv delta [_WRedEqInductionType] zeta
+    in _WRedEqInductionType in
+    let ind' := polymorphise ind in
+  exact ind').
+
+(* KM: looks like there is a bunch of polymorphic universes appearing there... *)
+Lemma WRedEqInduction : WRedEqInductionType.
+Proof.
+  intros PRedEq PPropEq **; split; now apply (_WRedEqInduction PRedEq PPropEq).
+Defined.
+
+End WRedTmEq.
+Arguments WRedTmEq {_ _ _ _ _ _ _ _ _ _ _ _} _ {_}.
+Arguments WPropEq {_ _ _ _ _ _ _ _ _ _ _ _} _ {_}.
+
+Section Lemmas.
+  Context `{GenericTypingProperties} {Γ A B} {WA : WRedTyPack Γ A B}.
+
+  Lemma wred_isW {Δ} {ρ : Δ ≤ Γ} {t u} : WPropEq WA ρ t u -> isW t <&> isW u.
   Proof.
-    intros [? ? ispair]; simpl; destruct ispair; constructor; tea.
-    now eapply convneu_whne.
+    intros [| ?? []]; split ; constructor.
+    all: eapply convneu_whne; tea; now symmetry.
   Qed.
 
-  Definition whred `{GenericTypingProperties} {Γ A B} {ΣA : SigRedTyPack Γ A B} {t} :
-    SigRedTm ΣA t -> [Γ |- t ↘  SigRedTyPack.outTy ΣA].
+  Lemma whredtm_both {Δ} {ρ : Δ ≤ Γ} {t u} : WRedTmEq WA ρ t u -> [Δ |- t ↘  (WRedTyPack.outTy WA)⟨ρ⟩ ] <&> [Δ |- u ↘  (WRedTyPack.outTy WA)⟨ρ⟩ ].
   Proof.
-    intros [?? ispair]; econstructor; tea.
-    destruct ispair; constructor; now eapply convneu_whne.
+    intros []; split; econstructor; tea;
+    eapply isW_whnf; [eapply nfst|eapply nsnd]; now eapply wred_isW.
   Defined.
 
-  Record SigRedTmEq `{ta : tag} `{WfContext ta}
-    `{WfType ta} `{ConvType ta} `{RedType ta}
-    `{Typing ta} `{ConvTerm ta} `{ConvNeuConv ta} `{RedTerm ta}
-    {Γ : context} {A B : term} {ΣA : SigRedTyPack Γ A B} {t u : term}
-  : Type := {
-    redL : SigRedTm ΣA t ;
-    redR : SigRedTm ΣA u ;
-    eq : [ Γ |- redL.(nf) ≅ redR.(nf) : SigRedTyPack.outTy ΣA ];
-    eqFst [Δ] (ρ : Δ ≤ Γ) (h : [ |- Δ ]) :
-      [ΣA.(PolyRedPack.shpRed) ρ h | Δ ||- tFst redL.(nf)⟨ρ⟩ ≅ tFst redR.(nf)⟨ρ⟩ : ΣA.(ParamRedTyPack.domL)⟨ρ⟩] ;
-    eqSnd [Δ] (ρ : Δ ≤ Γ) (h : [ |- Δ ]) :
-      [ΣA.(PolyRedPack.posRed) ρ h (eqFst ρ h) | Δ ||- tSnd redL.(nf)⟨ρ⟩ ≅ tSnd redR.(nf)⟨ρ⟩ : _] ;
-  }.
+  Lemma whredtm_both_id {t u} : WRedTmEq WA (@wk_id Γ) t u -> [Γ |- t ↘  (WRedTyPack.outTy WA) ] <&> [Γ |- u ↘  (WRedTyPack.outTy WA) ].
+  Proof.
+    intros [[] []]%whredtm_both; split; econstructor.
+    1,3: erewrite <-(wk_id_ren_on Γ (WRedTyPack.outTy _)); tea.
+    all: tea.
+  Defined.
 
-  Arguments SigRedTmEq {_ _ _ _ _ _ _ _ _ _ _ _}.
+End Lemmas.
 
-  Definition whredL `{GenericTypingProperties} {Γ A B} {ΣA : SigRedTyPack Γ A B} {t u} :
-    SigRedTmEq ΣA t u -> [Γ |- t ↘  SigRedTyPack.outTy ΣA ].
-  Proof. intros []; now eapply whred. Defined.
+End WRedTmEq.
 
-  Definition whredR `{GenericTypingProperties} {Γ A B} {ΣA : SigRedTyPack Γ A B} {t u} :
-    SigRedTmEq ΣA t u -> [Γ |- u ↘  SigRedTyPack.outTy ΣA ].
-  Proof. intros []; now eapply whred. Defined.
-
-End SigRedTmEq.
-
-Export SigRedTmEq(SigRedTm,Build_SigRedTm, SigRedTmEq,Build_SigRedTmEq).
+Export WRedTmEq(WRedTmEq,Build_WRedTmEq, WPropEq, WRedEqInduction).
