theories/LogicalRelation.v
@@ -1,2 +1,2 @@
 (** * LogRel.LogicalRelation: Definition of the logical relation *)
-From LogRel.LogicalRelation.Definition Require Export Prelude Ne Universe Poly Pi Sig Nat Empty Id Def Helper.
+From LogRel.LogicalRelation.Definition Require Export Prelude Ne Universe Poly Pi Sig Nat Empty Id W Def Helper.
